examples/metatheory/f-omega.fst
@@ -53,7 +53,7 @@ opaque type erenaming (s:esub) = (forall (x:var). is_EVar (s x))
 val is_erenaming : s:esub -> Tot (n:int{(  erenaming s  ==> n=0) /\
                                         (~(erenaming s) ==> n=1)})
 let is_erenaming s = (if excluded_middle (erenaming s) then 0 else 1)
-  (* not marking erenaming 'opaque' triggers #122 *)
+  (* not marking erenaming 'opaque' triggers #222 *)
 
 val esub_inc : var -> Tot exp
 let esub_inc y = EVar (y+1)
